cogent/examples/wa_connect/WordArray_StrCorresProof.thy
@@ -1,5 +1,5 @@
 theory WordArray_StrCorresProof
-  imports WordArray_CorresProof_Asm WordArray_SCCorres WordArray_UpdCCorres
+  imports WordArray_CorresProof_Asm  WordArray_UpdCCorres
 begin
 context WordArray begin
 
@@ -25,7 +25,7 @@ where
    (\<not> prod.snd (m s)) \<and>
    (\<forall>r' s'. (r',s') \<in> prod.fst (m s) \<longrightarrow>
      (\<exists>\<sigma>' r.(\<xi>', \<gamma> \<turnstile> (\<sigma>,c)  \<Down>! (\<sigma>',r)) \<and> (\<sigma>',s') \<in> srel \<and> val_rel r r')))"
-
+(*
 definition corres_shallow_C_strong where
   "corres_shallow_C_strong
      (rename' :: funtyp \<times> type list \<Rightarrow> funtyp)
@@ -52,6 +52,7 @@ definition corres_shallow_C_strong where
        (\<xi>\<^sub>v\<^sub>m, \<gamma>\<^sub>v\<^sub>m \<turnstile> prog\<^sub>m \<Down> val.rename_val rename' (val.monoval v\<^sub>p)) \<and>
        (\<sigma>', s') \<in> srel \<and>
        val_rel_shallow_C rename v\<^sub>s r' v\<^sub>p v\<^sub>u\<^sub>m \<xi>\<^sub>v\<^sub>p \<sigma>' \<Xi>\<^sub>m)))"
+*)
 
 section "Stronger Correspondence Lemmas/Theorems"
 
@@ -60,51 +61,33 @@ subsection "wordarray_put2"
 lemma upd_C_wordarray_put2_corres_strong:
 "\<And>i \<gamma> v' \<Gamma>' \<sigma> st.
     \<lbrakk>i < length \<gamma>; val_rel (\<gamma> ! i) v'; \<Gamma>' ! i = option.Some (prod.fst (prod.snd (\<Xi> ''wordarray_put2_0'')))\<rbrakk>
-    \<Longrightarrow> corres_strong (Generated.state_rel abs_repr_u) (App (AFun ''wordarray_put2_0'' []) (Var i))
+    \<Longrightarrow> corres_strong (Generated.state_rel wa_abs_repr) (App (AFun ''wordarray_put2_0'' []) (Var i))
          (do x <- main_pp_inferred.wordarray_put2_0' v';
              gets (\<lambda>s. x)
           od)
          \<xi>0 \<gamma> \<Xi>  \<Gamma>' \<sigma> st"
   apply (insert proc_ctx_wellformed_\<Xi> upd_proc_env_matches_ptrs_\<xi>0_\<Xi>)
   apply (unfold corres_strong_def)
-  apply (drule_tac i  = i  and 
+  apply (cut_tac i  = i  and 
                    \<gamma>  = \<gamma>  and 
                    v' = v' and
                    \<Gamma>' = \<Gamma>' and
                    \<sigma>  = \<sigma>  and
                    st = st in upd_C_wordarray_put2_corres; clarsimp simp: corres_def)
   done
-
-theorem shallow_C_wordarray_put2_corres_strong:
-"\<lbrakk>vv\<^sub>m = value_sem.rename_val rename (value_sem.monoval vv\<^sub>p);
- correspondence_init.val_rel_shallow_C abs_repr_u abs_upd_val' rename vv\<^sub>s uv\<^sub>C vv\<^sub>p uv\<^sub>m \<xi>p \<sigma> \<Xi>; 
- value_sem.matches abs_typing_v \<Xi> [vv\<^sub>m] [option.Some (prod.fst (prod.snd Generated_TypeProof.wordarray_put2_u32_type))]\<rbrakk>
-\<Longrightarrow> correspondence_init.corres_shallow_C abs_repr_u abs_typing_u abs_upd_val' rename (Generated.state_rel abs_repr_u)
-     (Generated_Shallow_Desugar.wordarray_put2_u32 vv\<^sub>s) Generated_TypeProof.wordarray_put2_u32
-     (main_pp_inferred.wordarray_put2_u32' uv\<^sub>C) \<xi>0 \<xi>m \<xi>p [uv\<^sub>m] [vv\<^sub>m] \<Xi>
-     [option.Some (prod.fst (prod.snd Generated_TypeProof.wordarray_put2_u32_type))] \<sigma> s"
-  apply (insert value_sem_rename_mono_prog_rename_\<Xi>_\<xi>m_\<xi>p 
-                val_proc_env_matches_\<xi>m_\<Xi> 
-                proc_env_u_v_matches_\<xi>0_\<xi>m_\<Xi>
-                proc_ctx_wellformed_\<Xi>
-                upd_C_wordarray_put2_corres
-                upd_proc_env_matches_ptrs_\<xi>0_\<Xi>)
-  apply (rule shallow_C_wordarray_put2_corres; simp)
-  done
-
 subsection "wordarray_length"
 
 lemma upd_C_wordarray_length_corres_strong:
 "\<And>i \<gamma> v' \<Gamma>' \<sigma> st.
     \<lbrakk>i < length \<gamma>; val_rel (\<gamma> ! i) v'; \<Gamma>' ! i = option.Some (prod.fst (prod.snd (\<Xi> ''wordarray_length_0'')))\<rbrakk>
-    \<Longrightarrow> corres_strong (Generated.state_rel abs_repr_u) (App (AFun ''wordarray_length_0'' []) (Var i))
+    \<Longrightarrow> corres_strong (Generated.state_rel wa_abs_repr) (App (AFun ''wordarray_length_0'' []) (Var i))
          (do x <- main_pp_inferred.wordarray_length_0' v';
              gets (\<lambda>s. x)
           od)
          \<xi>0 \<gamma> \<Xi>  \<Gamma>' \<sigma> st"
   apply (insert proc_ctx_wellformed_\<Xi> upd_proc_env_matches_ptrs_\<xi>0_\<Xi>)
   apply (unfold corres_strong_def)
-  apply (drule_tac i  = i  and 
+  apply (cut_tac i  = i  and 
                    \<gamma>  = \<gamma>  and 
                    v' = v' and
                    \<Gamma>' = \<Gamma>' and
@@ -112,58 +95,24 @@ lemma upd_C_wordarray_length_corres_strong:
                    st = st in upd_C_wordarray_length_corres; clarsimp simp: corres_def)
   done
 
-theorem shallow_C_wordarray_length_corres_strong:
-"\<lbrakk>vv\<^sub>m = value_sem.rename_val rename (value_sem.monoval vv\<^sub>p);
- correspondence_init.val_rel_shallow_C abs_repr_u abs_upd_val' rename vv\<^sub>s uv\<^sub>C vv\<^sub>p uv\<^sub>m \<xi>p \<sigma> \<Xi>;
- value_sem.matches abs_typing_v \<Xi> [vv\<^sub>m] [option.Some (prod.fst (prod.snd Generated_TypeProof.wordarray_length_u32_type))]\<rbrakk>
-\<Longrightarrow> correspondence_init.corres_shallow_C abs_repr_u abs_typing_u abs_upd_val' rename (Generated.state_rel abs_repr_u)
-     (Generated_Shallow_Desugar.wordarray_length_u32 vv\<^sub>s) Generated_TypeProof.wordarray_length_u32
-     (main_pp_inferred.wordarray_length_u32' uv\<^sub>C) \<xi>0 \<xi>m \<xi>p [uv\<^sub>m] [vv\<^sub>m] \<Xi>
-     [option.Some (prod.fst (prod.snd Generated_TypeProof.wordarray_length_u32_type))] \<sigma> s"
-  apply (insert value_sem_rename_mono_prog_rename_\<Xi>_\<xi>m_\<xi>p 
-                val_proc_env_matches_\<xi>m_\<Xi> 
-                proc_env_u_v_matches_\<xi>0_\<xi>m_\<Xi>
-                proc_ctx_wellformed_\<Xi>
-                upd_C_wordarray_length_corres
-                upd_proc_env_matches_ptrs_\<xi>0_\<Xi>)
-  apply (rule shallow_C_wordarray_length_corres; simp)
-  done
-
 subsection "wordarray_get"
 
 lemma upd_C_wordarray_get_corres_strong:
 "\<And>i \<gamma> v' \<Gamma>' \<sigma> st.
     \<lbrakk>i < length \<gamma>; val_rel (\<gamma> ! i) v'; \<Gamma>' ! i = option.Some (prod.fst (prod.snd (\<Xi> ''wordarray_get_0'')))\<rbrakk>
-    \<Longrightarrow> corres_strong (Generated.state_rel abs_repr_u) (App (AFun ''wordarray_get_0'' []) (Var i))
+    \<Longrightarrow> corres_strong (Generated.state_rel wa_abs_repr) (App (AFun ''wordarray_get_0'' []) (Var i))
          (do x <- main_pp_inferred.wordarray_get_0' v';
              gets (\<lambda>s. x)
           od)
          \<xi>0 \<gamma> \<Xi>  \<Gamma>' \<sigma> st"
   apply (insert proc_ctx_wellformed_\<Xi> upd_proc_env_matches_ptrs_\<xi>0_\<Xi>)
   apply (unfold corres_strong_def)
-  apply (drule_tac i  = i  and 
+  apply (cut_tac i  = i  and 
                    \<gamma>  = \<gamma>  and 
                    v' = v' and
                    \<Gamma>' = \<Gamma>' and
                    \<sigma>  = \<sigma>  and
                    st = st in upd_C_wordarray_get_corres; clarsimp simp: corres_def)
-  done
-
-theorem shallow_C_wordarray_get_strong:
-"\<lbrakk>vv\<^sub>m = value_sem.rename_val rename (value_sem.monoval vv\<^sub>p);
- correspondence_init.val_rel_shallow_C abs_repr_u abs_upd_val' rename vv\<^sub>s uv\<^sub>C vv\<^sub>p uv\<^sub>m \<xi>p \<sigma> \<Xi>;
- value_sem.matches abs_typing_v \<Xi> [vv\<^sub>m] [option.Some (prod.fst (prod.snd Generated_TypeProof.wordarray_get_u32_type))]\<rbrakk>
-\<Longrightarrow> correspondence_init.corres_shallow_C abs_repr_u abs_typing_u abs_upd_val' rename (Generated.state_rel abs_repr_u)
-     (Generated_Shallow_Desugar.wordarray_get_u32 vv\<^sub>s) Generated_TypeProof.wordarray_get_u32
-     (main_pp_inferred.wordarray_get_u32' uv\<^sub>C) \<xi>0 \<xi>m \<xi>p [uv\<^sub>m] [vv\<^sub>m] \<Xi>
-     [option.Some (prod.fst (prod.snd Generated_TypeProof.wordarray_get_u32_type))] \<sigma> s"
-  apply (insert value_sem_rename_mono_prog_rename_\<Xi>_\<xi>m_\<xi>p 
-                val_proc_env_matches_\<xi>m_\<Xi> 
-                proc_env_u_v_matches_\<xi>0_\<xi>m_\<Xi>
-                proc_ctx_wellformed_\<Xi>
-                upd_C_wordarray_get_corres
-                upd_proc_env_matches_ptrs_\<xi>0_\<Xi>)
-  apply (rule shallow_C_wordarray_get_corres; simp)
   done
 
 end (* end of context *)
